proof/spec/KyberProperties.ec
@@ -4,8 +4,6 @@ require import Array32 Array64 Array128 Array168 Array256 Array384.
 require import Array768 Array960 Array1024 Array1152.
 require import Kyber.
 
-import KMatrix.
-import KyberPKE.
 (**********************************)
 (**********************************)
 (**********************************)
@@ -50,11 +48,30 @@ phoare sem_decode10_vec a : [ EncDec.decode10_vec : arg = a ==> res = sem_decode
 phoare sem_encode12_vec a : [ EncDec.encode12_vec : arg = a ==> res = sem_encode12_vec a ] = 1%r by admit. (* reify *)
 phoare sem_encode10_vec a : [ EncDec.encode10_vec : arg = a ==> res = sem_encode10_vec a ] = 1%r by admit. (* reify *)
 
+(**************************************************************************
+   MLWE_PKE is the theory where we prove an abstract PKE construction
+   that matches the algebraic basis of Kyber. This theory clones MLWE
+   to get the hard problem definitions, and so it gets a bunch of 
+   theories and RO clones. 
+   We are interested in a sub-theory called MLWE_PKE_GENERAL, which 
+   is the one for which we prove the most general results for 
+   Kyber. Within it, we must fix the RO_SMP clone.
 
-(**********************************)
+   It also independently clones PKE_Ext as PKE_, but it already fixes
+   the underlying RO to MLWE_.RO_SMP, so all we need to fix is RO_SMP in 
+   the MWLW_.RO_SMP. 
+
+   This clone gives us the security proofs for the algebraic version
+   of KyberPKE. To get proofs for Kyber spec, we just need to explain
+   how the Kyber spec functionally maps to this algebraic version
+   and then derive the properties as corollaries.
+***************************************************************************)
 require (****) MLWE_PKE.
 
 theory SpecProperties.
+
+import KMatrix.
+import KyberPKE.
 
 type pkey = W8.t Array1152.t * W8.t Array32.t.
 type skey = W8.t Array1152.t.  
@@ -73,9 +90,23 @@ op c_decode(c : ciphertext) =
 op rnd_err_v = compress_poly_err 4. 
 op rnd_err_u = mapv (compress_poly_err 10). 
 
+op max_noise = q %/ 4.
+
+op pe_R = pe^256.
+op pv = pe_R^(kvec).
+op pm = pe_R^(kvec^2).
+
+op under_noise_bound (p : poly) (b : int) =
+     all (fun cc => `| as_sint cc| < b) p.
+
+op cv_bound : int = 104. (* this is the compress error bound for d = 4 *)
+op fail_prob : real. (* Need to compute exact value or replace
+                        with suitable bound *)
+
+op epsilon_hack : real. (* Assumed simplification loss *)
+
 clone import MLWE_PKE as MLWEPKE with 
-  type MLWE_.MLWE_SMP.RO_SMP.in_t = W8.t Array32.t * W8.t * W8.t * int,
-  type MLWE_.MLWE_SMP.RO_SMP.out_t = W8.t Array168.t,
+  theory MLWE_PKE_GENERAL.MLWE_SMP.RO_SMP <- RO,
   type MLWE_.Matrix_.R = poly,
   type MLWE_.Matrix_.Matrix.matrix <- matrix,
   type MLWE_.Matrix_.vector <- vector,
@@ -88,6 +119,7 @@ clone import MLWE_PKE as MLWEPKE with
   op MLWE_.Matrix_.ZR.( * ) <- Poly.(&*),
   op MLWE_.Matrix_.ZR.invr <- KMatrix.ZR.invr,
   op MLWE_.Matrix_.size <- kvec,
+  op MLWE_.Matrix_.Vector.(+) <- KMatrix.Vector.(+),
   op MLWE_.Matrix_.Vector.prevector <- prevector,
   op MLWE_.Matrix_.Vector.vclamp <- vclamp,
   op MLWE_.Matrix_.Vector.tofunv <- tofunv,
@@ -167,15 +199,13 @@ admitted.
 realize sk_encodeK.
 admitted.
 
-
-(*
-realize encode_noise.
+realize MLWE_PKE_RO.Correctness.encode_noise.
 move => /> u v.
 rewrite /c_decode /c_encode /rnd_err_u /rnd_err_v /= sem_encode10_vecK sem_encode4K => />.
 split; last  by rewrite round_poly_errE.
 rewrite /(+) /mapv /=.
 apply eq_vectorP => /> i il ih; rewrite !offunvE 1,2:/# /=.
-rewrite MLWE_.Matrix_.Vector.offunvE 1:/# /= /compress_poly_err /=.
+rewrite Vector.offunvE 1:/# /= /compress_poly_err /=.
 apply Array256.tP => k kb.
 rewrite /compress_polyvec /= /fromarray256 /= /Poly.(&+) /=.
 rewrite mapiE // map2E //= initiE //= initiE //= mapiE //= 1:/# initiE 1:/# /=. 
@@ -183,35 +213,35 @@ rewrite decompress_errE //; 1: smt(qE).
 by rewrite mapiE /#.
 qed.
 
-realize good_decode. 
+realize MLWE_PKE_RO.Correctness.good_decode. 
 rewrite /under_noise_bound /m_encode /m_decode /compress_poly /decompress_poly  => m n hgood.
 have : sem_decode1 (sem_encode1 (map (compress 1) (map (decompress 1) (sem_decode1 m) &+ n))) = (sem_decode1 m); last by smt(sem_decode1K).
 apply Array256.ext_eq => /> x h0x hx256. 
 rewrite sem_encode1K /(&+) mapiE 1:/# map2E /= initiE /= 1:/# mapiE 1:/#.
 rewrite b_decode_sem /b_decode /= -decompress_alt_decompress // /decompress_alt /= qE /=.
 rewrite /as_sint => />.
-rewrite Zq.addE  qE inFqK qE => />.
-admitted. (* what's going on *)
+rewrite Zq.addE  qE Zq.inFqK qE => />.
+admitted. (* lost track of what is going on *)
 
-realize cv_bound_valid.
+realize MLWE_PKE_RO.Correctness.cv_bound_valid.
 admitted. (* Rounding upper bound for one coefficient: compute in EC? *)
 
-realize noise_commutes.
+realize MLWE_PKE_RO.Correctness.noise_commutes.
 move => n n' b H H0.
 move : H H0; rewrite /under_noise_bound.
 rewrite !allP.
 move => Hn Hnp i ib.
 move : (Hn i ib). 
 move : (Hnp i ib) => /=. 
-rewrite /as_sint /Poly.(&+) /= map2E !initiE //= addE qE /=  !StdOrder.IntOrder.ltr_norml /= => Hni Hnpi.
+rewrite /as_sint /Poly.(&+) /= map2E !initiE //= Zq.addE qE /=  !StdOrder.IntOrder.ltr_norml /= => Hni Hnpi.
 by smt().
 qed.
 
-realize correctness_hack.
+realize MLWE_PKE_RO.Correctness.correctness_hack.
 admitted. (* assumption: no one knows what this bound is *)
 
 
-realize fail_prob.
+realize MLWE_PKE_RO.Correctness.fail_prob.
 move => &m;byphoare.
 proc.
 auto => />.
@@ -219,146 +249,17 @@ rewrite /comp_distr /noise_exp_final /noise_exp_part /rdistr.
 rewrite /good_noise /cv_bound /noise_val.
 admitted. (* Probability of failure event in distribution: compute in EC? *)
 
-*)
+(* We now specify the various components used by Kyber spec so that 
+   we can relate it to the abstract construction. The differences
+   are only in the sampling procedures. *)
+import MLWE_PKE_GENERAL.
 
-(**********************************)
-(**********************************)
-(**********************************)
-(* We need to modularize the 
-   matrix sampler*)
-(**********************************)
-(**********************************)
-(**********************************)
-
-module Kyber(G : G_t, XOF : XOF_t, PRF : PRF_t, O : RO.POracle, S : Sampler) : Scheme = {
-
-
-
-  (* Spec gives a derandomized enc that matches this code *)
-  proc kg_derand(seed: W8.t Array32.t) : pkey * skey = {
-     var rho, sig, i, j, _N,c,t;
-     var tv,sv : W8.t Array1152.t;
-     var a : matrix;
-     var s,e : vector;
-     a <- witness;
-     e <- witness;
-     s <- witness;
-     sv <- witness;
-     tv <- witness;
-     (rho,sig) <@ G(O).sample(seed);
-     _N <- 0; 
-     i <- 0;
-     while (i < kvec) {
-        j <- 0;
-        while (j < kvec) {
-           XOF(O).init(rho,W8.of_int j,W8.of_int i);
-           c <@ Parse(XOF,O).sample_real();
-           a.[(i,j)] <- c;
-           j <- j + 1;
-        }
-        i <- i + 1;
-     }      
-     PRF(O).init(sig);
-     i <- 0;
-     while (i < kvec) {
-        c <@ CBD2(PRF,O).sample_real(_N);
-        s <- set s i c;
-        _N <- _N + 1;
-        i <- i + 1;
-     }         
-     i <- 0;
-     while (i < kvec) {
-        c <@ CBD2(PRF,O).sample_real(_N);
-        e <- set e i c;
-        _N <- _N + 1;
-        i <- i + 1;
-     }      
-     s <- nttv s;
-     e <- nttv e; 
-     t <- ntt_mmul a s + e;
-     tv <@ EncDec.encode12_vec(toipolyvec t); (* minimum residues *)
-     sv <@ EncDec.encode12_vec(toipolyvec s); (* minimum residues *)
-     return ((tv,rho),sv);
-  }
-
-  proc kg() : pkey * skey = {
-     var s,kp;
-     s <$ srand;
-     kp <@ kg_derand(s);
-     return kp;
-  }
-
-  (* Spec gives a derandomized enc that matches this code *)
-  proc enc_derand(pk : pkey, m : plaintext, r : W8.t Array32.t) : ciphertext = {
-      var _N,i,j,c,tv,rho,rv,e1,e2,rhat,u,v,mp,c2,thati;
-      var that : vector;
-      var aT : matrix;
-      var c1 : W8.t Array960.t;
-      aT <- witness;
-      c1 <- witness;
-      e1 <- witness;
-      rv <- witness;
-      that <- witness;
-      (tv,rho) <- pk;
-      _N <- 0;
-      thati <@ EncDec.decode12_vec(tv); 
-      that <- ofipolyvec thati;
-      i <- 0;
-      while (i < kvec) {
-        j <- 0;
-        while (j < kvec) {
-           XOF(O).init(rho,W8.of_int i, W8.of_int j);
-           c <@ Parse(XOF,O).sample_real();
-           aT.[(i,j)] <- c; (* this is the transposed matrix *)
-           j <- j + 1;
-        }
-        i <- i + 1;
-      } 
-      PRF(O).init(r);     
-      i <- 0;
-      while (i < kvec) {
-        c <@ CBD2(PRF,O).sample_real(_N);
-        rv <- set rv i c;
-        _N <- _N + 1;
-        i <- i + 1;
-      }         
-      i <- 0;
-      while (i < kvec) {
-        c <@ CBD2(PRF,O).sample_real(_N);
-        e1 <- set e1 i c;
-        _N <- _N + 1;
-        i <- i + 1;
-      }      
-      e2 <@ CBD2(PRF,O).sample_real(_N);
-      rhat <- nttv rv;
-      u <- invnttv (ntt_mmul aT rhat) + e1;
-      mp <@ EncDec.decode1(m);
-      v <- invntt (ntt_dotp that rhat) &+ e2 &+ decompress_poly 1 mp; 
-      c1 <@ EncDec.encode10_vec(compress_polyvec 10 u); 
-      c2 <@ EncDec.encode4(compress_poly 4 v);
-      return (c1,c2);
-  }
-
-  proc enc(pk : pkey, m : plaintext) : ciphertext = {
-     var r,c;
-     r <$ srand;
-     c <@ enc_derand(pk,m,r);
-     return c;
-  }
-
-  include Kyber[dec]
-}.
-
-
-
-(* We now specify the various components used by Kyber in the ROM *)
-
+op SHA3_SMOOTH : W8.t Array32.t -> W8.t Array32.t * W8.t Array32.t.
 
 module (G : G_t) (O : RO.POracle) = {
    proc sample(seed : W8.t Array32.t) : (W8.t Array32.t) *  (W8.t Array32.t) = {
         var rho, sig : W8.t Array32.t;
-        rho <$ srand;
-        sig <$ srand;
+        (rho,sig) <- SHA3_SMOOTH seed;
         return (rho,sig);
    }
 }.
@@ -404,10 +305,7 @@ module (PRF : PRF_t) (O : RO.POracle) = {
    }
 }.
 
-(* These modules are reductions. They just encode/decode things coming from the
-   refined game to the scheme adversary.  *)
-
-module (S : MLWE_.Sampler) (O : MLWE_.MLWE_SMP.RO_SMP.POracle)  = {
+module (KSampler(XOF : XOF_t) : MLWE_SMP.Sampler) (O : RO.POracle)  = {
     proc sample(sd : W8.t Array32.t) : matrix = { 
      var i,j,c;
      var a : matrix;
@@ -427,41 +325,221 @@ module (S : MLWE_.Sampler) (O : MLWE_.MLWE_SMP.RO_SMP.POracle)  = {
     }
 }.
 
+(*************************************
+We define a version of Kyber spec that
+uses a sampler. This is useful for 
+syntactic reasons.
+*************************************)
+
+
+module KyberS(G : G_t, S : MLWE_SMP.Sampler, PRF : PRF_t, O : RO.POracle) : Scheme = {
+
+  (* Spec gives a derandomized enc that matches this code *)
+  proc kg_derand(seed: W8.t Array32.t) : pkey * skey = {
+     var rho, sig, i,  _N,c,t;
+     var tv,sv : W8.t Array1152.t;
+     var a : matrix;
+     var s,e : vector;
+     e <- witness;
+     s <- witness;
+     sv <- witness;
+     tv <- witness;
+     (rho,sig) <@ G(O).sample(seed);
+     _N <- 0; 
+     a <@ S(O).sample(rho);     
+     PRF(O).init(sig);
+     i <- 0;
+     while (i < kvec) {
+        c <@ CBD2(PRF,O).sample_real(_N);
+        s <- set s i c;
+        _N <- _N + 1;
+        i <- i + 1;
+     }         
+     i <- 0;
+     while (i < kvec) {
+        c <@ CBD2(PRF,O).sample_real(_N);
+        e <- set e i c;
+        _N <- _N + 1;
+        i <- i + 1;
+     }      
+     s <- nttv s;
+     e <- nttv e; 
+     t <- ntt_mmul a s + e;
+     tv <@ EncDec.encode12_vec(toipolyvec t); (* minimum residues *)
+     sv <@ EncDec.encode12_vec(toipolyvec s); (* minimum residues *)
+     return ((tv,rho),sv);
+  }
+
+  proc kg() : pkey * skey = {
+     var s,kp;
+     s <$ srand;
+     kp <@ kg_derand(s);
+     return kp;
+  }
+
+  (* Spec gives a derandomized enc that matches this code *)
+  proc enc_derand(pk : pkey, m : plaintext, r : W8.t Array32.t) : ciphertext = {
+      var _N,i,c,tv,rho,rv,e1,e2,rhat,u,v,mp,c2,thati;
+      var that : vector;
+      var aT : matrix;
+      var c1 : W8.t Array960.t;
+      aT <- witness;
+      c1 <- witness;
+      e1 <- witness;
+      rv <- witness;
+      that <- witness;
+      (tv,rho) <- pk;
+      _N <- 0;
+      thati <@ EncDec.decode12_vec(tv); 
+      that <- ofipolyvec thati;
+      aT <@ S(O).sample(rho);    
+      aT <- trmx aT; 
+      PRF(O).init(r);     
+      i <- 0;
+      while (i < kvec) {
+        c <@ CBD2(PRF,O).sample_real(_N);
+        rv <- set rv i c;
+        _N <- _N + 1;
+        i <- i + 1;
+      }         
+      i <- 0;
+      while (i < kvec) {
+        c <@ CBD2(PRF,O).sample_real(_N);
+        e1 <- set e1 i c;
+        _N <- _N + 1;
+        i <- i + 1;
+      }      
+      e2 <@ CBD2(PRF,O).sample_real(_N);
+      rhat <- nttv rv;
+      u <- invnttv (ntt_mmul aT rhat) + e1;
+      mp <@ EncDec.decode1(m);
+      v <- invntt (ntt_dotp that rhat) &+ e2 &+ decompress_poly 1 mp; 
+      c1 <@ EncDec.encode10_vec(compress_polyvec 10 u); 
+      c2 <@ EncDec.encode4(compress_poly 4 v);
+      return (c1,c2);
+  }
+
+  proc enc(pk : pkey, m : plaintext) : ciphertext = {
+     var r,c;
+     r <$ srand;
+     c <@ enc_derand(pk,m,r);
+     return c;
+  }
+
+  proc dec(sk : skey, cph : ciphertext) : plaintext option = {
+      var m,mp,ui,v,vi,si, c1, c2;
+      var u,s : vector;
+      u <- witness;
+      s <- witness;
+      (c1,c2) <- cph;
+      ui <@ EncDec.decode10_vec(c1);
+      u <- decompress_polyvec 10 ui;
+      vi <@ EncDec.decode4(c2);
+      v <- decompress_poly 4 vi;
+      si <@ EncDec.decode12_vec(sk);
+      s <- ofipolyvec si;
+      mp <- v &+ ((&-) (invntt (ntt_dotp s (nttv u))));
+      m <@ EncDec.encode1(compress_poly 1 mp);
+      return Some m;
+  }
+
+}.
+
+equiv kg_sampler_kg (O <: RO.POracle) :
+   KyberS(G,KSampler(XOF),PRF,O).kg ~ Kyber(G,XOF,PRF,O).kg : ={arg} /\ ={glob O} ==> ={res}.
+proc;inline*.
+seq 12 11: (#pre /\ ={sig} /\ ={s0} /\ ={rho} /\ ={e} /\ a0{1} = a{2} /\ ={_N} /\ sd{1} = rho{2}); 1: by auto.
+sim => />. admitted. (* sim does not understand extensional equality *)
+
+equiv enc_sampler_enc (O <: RO.POracle) :
+   KyberS(G,KSampler(XOF),PRF,O).enc ~ Kyber(G,XOF,PRF,O).enc : ={arg} /\ ={glob O} ==> ={res}.
+proc;inline*. 
+seq 31 29: (#pre /\ ={that, rv, r0, m0, e1, aT, _N}); 1: by sim.
+sim => />. admitted. (* sim does not understand extensional equality or transposition. *)
+
+equiv enc_sampler_dec (O <: RO.POracle) :
+   KyberS(G,KSampler(XOF),PRF,O).dec ~ Kyber(G,XOF,PRF,O).dec : ={arg} /\ ={glob O} ==> ={res} by proc;inline *;sim => /#.
+
 (***************************************)
 
 section.
 
-declare module As <: KyberPKE.AdversaryRO {-MLWE_.MLWE_SMP.RO_SMP.Lazy.LRO,-RO.Lazy.LRO, -XOF, -PRF}.
+declare module O <: RO.Oracle {-PRF, -B1ROM, -B2ROM}.
+declare module S <: MLWE_SMP.Sampler {-PRF, -O, -B1ROM, -B2ROM}.
+declare module As <: KyberPKE.AdversaryRO {-O, -S, -PRF, -B1ROM, -B2ROM}.
 
-lemma wrap_equiv_security &m :  
-  Pr[ KyberPKE.CPAGameROM(KyberPKE.CPA,MLWE_PKE(S(KyberPKE.RO.Lazy.LRO)),As,KyberPKE.RO.Lazy.LRO).main() @ &m : res] =
-  Pr[ KyberPKE.CPAGameROM(KyberPKE.CPA,Kyber(G,XOF,PRF),As,KyberPKE.RO.Lazy.LRO).main() @ &m : res].
+lemma security_any_sampler &m :  
+  islossless O.init =>
+  islossless O.o =>
+  (forall (x : RO.in_t), is_lossless (RO.dout x)) =>
+  (forall (O0 <: RO.Oracle), islossless O0.o => islossless S(O0).sample) =>
+  (forall (O0 <: RO.Oracle), islossless O0.o => islossless As(O0).guess) =>
+  (forall (O0 <: RO.Oracle), islossless O0.o => islossless As(O0).choose) =>
+  Pr[ KyberPKE.CPAGameROM(KyberPKE.CPA,KyberS(G,S,PRF),As,O).main() @ &m : res] - 1%r/2%r = 
+  Pr[MLWE_SMP.MLWE_SMP(B1ROM(As, S), S, O).main(false, false) @ &m : res] -
+ Pr[MLWE_SMP.MLWE_SMP(B1ROM(As, S), S, O).main(false, true) @ &m : res] +
+ Pr[MLWE_SMP.MLWE_SMP(B2ROM(As, S), S, O).main(true, false) @ &m : res] -
+ Pr[MLWE_SMP.MLWE_SMP(B2ROM(As, S), S, O).main(true, true) @ &m : res].
+move => H H0 H1 H2 H3 H4.
+have  <- : 
+    Pr[ PKE_.CPAGameROM(PKE_.CPA,MLWE_PKE(S(O)),As,O).main() @ &m : res] =
+    Pr[ KyberPKE.CPAGameROM(KyberPKE.CPA,KyberS(G,S,PRF),As,O).main() @ &m : res]; last by
+        apply (main_theorem_s O S As &m  H H0 H1 H2 H3 H4).
 byequiv => //.
 proc.
 inline {1} 2.
 inline {2} 2.
-wp;call(_: ={glob RO.Lazy.LRO}); 1: by sim.
-call(_: ={glob G, glob XOF, glob PRF, glob RO.Lazy.LRO}).
+wp;call(_: ={glob O}); 1: by sim.
+call(_: ={glob S, glob O}).
+(* ENCRYPTION IS EQUIVALENT: Write aux lemma.  *)
 + inline {2} 2.
   wp;ecall{2}(sem_encode4 (compress_poly 4 v{2})).
-admitted. (* wrapped abstract spec equiv to spec: security *)
+  wp;ecall{2}(sem_encode10_vec (compress_polyvec 10 u{2})).
+  wp;ecall{2}(sem_decode1 (m0{2})).
+  swap {1} 5 -3. (* follows from PRF hop and product of distributions *)
+  admit.
 
-(* 
-lemma KyberSecurity &m :
-  Pr[ KyberPKE.CPAGameROM(KyberPKE.CPA,Kyber(G,XOF,PRF),As,KyberPKE.RO.Lazy.LRO).main() @ &m : res] - 1%r / 2%r =
-      Pr[MLWE_.MLWE(MLWE_.B(B1ROM(Bs(As)), MLWE_.MLWE_SMP.RO_SMP.Lazy.LRO)).main(false) @ &m : res] -
-      Pr[MLWE_.MLWE(MLWE_.B(B1ROM(Bs(As)), MLWE_.MLWE_SMP.RO_SMP.Lazy.LRO)).main(true) @ &m : res] +
-      Pr[MLWE_.MLWE(MLWE_.Bt(B2ROM(Bs(As)), MLWE_.MLWE_SMP.RO_SMP.Lazy.LRO)).main(false) @ &m : res] -
-      Pr[MLWE_.MLWE(MLWE_.Bt(B2ROM(Bs(As)), MLWE_.MLWE_SMP.RO_SMP.Lazy.LRO)).main(true) @ &m : res].
-rewrite -wrap_equiv_security.
-rewrite (wrap_security &m).
-apply (main_theorem_h (Bs(As))). 
-admit. (* lossless *)
-admit. (* lossless *)
+rnd;call(_: ={glob O}); 1: by sim.
+conseq />; 1: by smt().
+
+(* KEYGEN IS EQUIVALENT: Write aux lemma.  *)
+call(_: ={glob S, glob O}).
+inline {2} 2. 
+wp;ecall{2}(sem_encode12_vec (toipolyvec s0{2})).
+wp;ecall{2}(sem_encode12_vec (toipolyvec t{2})).
+swap {1} 4 -2. 
+inline {2} 7.
+swap {2} [7..9] -4. 
+swap {2} 11 -5. 
+
+(* follows from PRF hop, entropy smoothing of SHA3_SMOOTH 
+   and product of distributions *)
+admit.
+
+by inline *; conseq => />; sim.
+
 qed.
 
-*)
 end section.
 
+(* TO DO: Derive the following results will require some
+changes to the Spec file, leaving the RO abstract there
+and fixing it only in cloning here *)
+
+section.
+
+(* Do the same for the MLWE based security theorem *)
+print MLWEPKE.MLWE_PKE_RO.Security.main_theorem_ro.
+
+end section.
+
+section.
+
+(* Do the same for correctness *)
+
+(* Do the same for the MLWE based security theorem *)
+print MLWEPKE.MLWE_PKE_RO.Correctness.correctness_bound.
+
+end section.
 
 end SpecProperties.
